finished proving problem 3.19

Lamda2.v
@@ -8,8 +8,8 @@ Definition atomic_type := nat.
 Inductive type : Type :=
 (* Defenition 3.4 *)
 | Var : atomic_type -> type
-| Arr : type -> type -> type
-| Pi : atomic_type -> type -> type.
+| Arr : type -> type -> type (*T2 → T2*)
+| Pi : atomic_type -> type -> type. (*ΠV : ∗ . T2)*)
 
 Infix ">>" := Arr (right associativity, at level 9).
 Notation "$" := Var (right associativity, at level 10).
@@ -18,18 +18,18 @@ Definition atomic_term : Type := nat.
 
 Inductive term : Type :=
 (* Defenition 3.4.1 *)
-| TVar : atomic_term -> term
-| App : term -> term -> term
-| Tapp : term -> type -> term
-| Abs : atomic_term -> type -> term -> term
-| Tabs : atomic_type -> type -> term.
+| TVar : atomic_term -> term (*V*)
+| App : term -> term -> term (*ΛΛ*)
+| Tapp : term -> type -> term (*ΛT2*)
+| Abs : atomic_term -> type -> term -> term (*λV : T2 . Λ)*)
+| Tabs : atomic_type -> term -> term. (*λV : ∗ . Λ)*)
 
 Infix "!" := (App) (left associativity, at level 11).
 Infix "!!" :=  (Tapp) (left associativity, at level 12).
-Notation "_\ x t m" :=
+(* Notation "-\ x t m" :=
     (Abs x t m)
     (at level 13, right associativity)
-    .
+    . *)
 Notation "*\ t m" :=
     (Tabs t m)
     (at level 14, right associativity)
@@ -91,16 +91,22 @@ Fixpoint type_eqb (a : type) (b : type): bool :=
 
 Compute (type_eqb ((Var 2) >> $3) (($2) >> $3)).
 Compute (type_eqb ($ 2) (Pi (3) ($3))).
-Fixpoint check_declaration (G : context) (x : atomic_term) (a : type) :
+Fixpoint check_declaration (G : context) (x' : term) (a : type) :
     bool :=
-        match G with
-        | [] => false
-        | d :: G' =>
-         match d with
-         |Sttd y b => (eqb x y && type_eqb a b) || check_declaration G' x a
-         | Std _ => check_declaration G' x a
-         end
+        match x' with
+        |TVar x =>
+            match G with
+            | [] => false
+            | d :: G' =>
+                match d with
+                |Sttd y b => (eqb x y && type_eqb a b) || check_declaration G' x' a
+                | Std _ => check_declaration G' x' a
+                end
+            end
+        | _ => false
         end.
+
+Compute check_declaration ([Sttd 3 ($ 2)]) (TVar 3) ($2).
 
 Fixpoint FVl (t : type) : list atomic_type :=
     match t with
@@ -109,18 +115,75 @@ Fixpoint FVl (t : type) : list atomic_type :=
     | Pi n t => remove PeanoNat.Nat.eq_dec n (FVl t)
     end.
 
+Fixpoint type_subst (t : type) (a : atomic_type) (b : type): type :=
+    match t with
+    | Var m =>
+        match eqb a m with
+        | true => b
+        | false => Var m
+        end
+    | m >> n => (type_subst m a b) >> (type_subst n a b)
+    | Pi n t => 
+        match (eqb n a) with
+        | true => Pi n t
+        | false => Pi n (type_subst t a b)
+        end
+    end.
 Definition foreach {T : Type} (l : list T) (P : T -> bool) :=
 fold_left andb (map P l) true = true.
 
 Inductive l2_context : context -> Prop :=
-| Emp : l2_context []
+| Emp : l2_context [] 
+(*∅ is a λ2-context;
+dom(∅) = ( ), the empty list.*)
 | l2T : forall (G : context) (a : atomic_type) , (l2_context G) ->
 (check_type G a = false) -> l2_context ( (Std a) :: G)
+(*If Γ is a λ2-context, α ∈ V and α not∈ dom(Γ), then Γ, α : ∗ is a λ2-context;
+dom(Γ, α : ∗) = (dom(Γ), α), i.e. dom(Γ) concatenated with α.*)
 | l2t : forall (G : context) (x : atomic_term) (r : type),
 l2_context G -> (check_term G x = false) ->
 (foreach (FVl r) (check_type G)) -> l2_context ((Sttd x r) :: G).
+(*If Γ is a λ2-context, if ρ ∈ T2 such that α ∈ dom(Γ) for all free type variables
+α occurring in ρ and if x not∈ dom(Γ), then Γ, x : ρ is a λ2-context;
+dom(Γ, x : ρ) = (dom(Γ), x).*)
 
-(* Inductive l2_legal : context -> term -> type -> Prop :=
+Inductive l2_legal : context -> statement -> Prop :=
+(*(var) Γ |- x : σ if Γ is a λ2-context and x : σ ∈ Γ*)
 | lvar : forall (G : context) (x : term) (a : type),
-(l2_context G) -> 
-. *)
+(l2_context G) ->  ((check_declaration G x a) = true) -> (l2_legal G (Stt x a))
+(* (form) Γ |- B : ∗ if Γ is a λ2-context, B ∈ T2 and
+all free type variables in B are declared in Γ *)
+| lform : forall (G: context) (B : type),
+l2_context G -> (foreach (FVl B) (check_type G)) -> l2_legal G (St B)
+(*(appl) Γ |- M : σ → τ, Γ |- N : σ
+Γ |- MN : τ*)
+| lappl : forall (G: context) (M N : term) (a t : type),
+(l2_legal G (Stt M (a >> t))) -> (l2_legal G (Stt N a)) -> l2_legal G (Stt (M ! N) a)
+(* (abst) Γ, x : σ |- M : τ
+Γ |- λx : σ . M : σ → τ*)
+| labst : forall (G: context) (x: atomic_term) (a t : type) (M : term),
+(l2_legal ((Sttd x a) :: G) (Stt M t)) -> (l2_legal G (Stt (Abs x a M) (a >> t)))
+(* (abst2) Γ, α :∗ |- M : A
+Γ |- λα : ∗. M : Πα : ∗. A*)
+| labst2 : forall (G: context) (a: atomic_type) (M : term) (A : type),
+(l2_legal ((Std a) :: G) (Stt M A)) -> l2_legal G (Stt (Tabs a M) (Pi a A))
+(*(appl2) Γ |- M : (Πα : ∗. A), Γ |- B : ∗
+Γ |- MB : A[α := B]*)
+| lappl2 : forall (G: context) (a: atomic_type) (M : term) (A B: type),
+(l2_legal G (Stt M (Pi a A))) -> l2_legal G (St B) -> l2_legal G (Stt (Tapp M B) (type_subst A a B)) 
+
+.
+
+Theorem nineteen: forall (G: context) (s: statement), l2_legal G s -> l2_context G.
+(*problem 19 in the book
+Prove: if Γ |- L : σ, then Γ is a λ2-context*)
+Proof.
+    intros. induction H.
+    - apply H.
+    - apply H.
+    - apply IHl2_legal1.
+    - inversion IHl2_legal. apply H3.
+    - inversion IHl2_legal. apply H2.
+    - apply IHl2_legal2.
+    
+Qed.
